add pairs

src/SourceLang.v
@@ -17,13 +17,14 @@ Definition type_eq_dec (t1 t2 : type) : {t1 = t2} + {t1 <> t2}.
 Defined.
 
 Inductive constr_type : constr_name -> list type -> type_name -> Type :=
-| CTS         : constr_type CS         [ADT Tnat]                  Tnat
-| CTO         : constr_type CO         []                          Tnat
-| CTtrue      : constr_type Ctrue      []                          Tbool
-| CTfalse     : constr_type Cfalse     []                          Tbool
-| CTnil ty    : constr_type Cnil       []                          (Tlist ty)
-| CTcons ty   : constr_type Ccons      [ADT ty; ADT (Tlist ty)]   (Tlist ty)
-| CTtt        : constr_type Ctt        []                          Tunit
+| CTS            : constr_type CS         [ADT Tnat]                  Tnat
+| CTO            : constr_type CO         []                          Tnat
+| CTtrue         : constr_type Ctrue      []                          Tbool
+| CTfalse        : constr_type Cfalse     []                          Tbool
+| CTnil ty       : constr_type Cnil       []                          (Tlist ty)
+| CTcons ty      : constr_type Ccons      [ADT ty; ADT (Tlist ty)]    (Tlist ty)
+| CTtt           : constr_type Ctt        []                          Tunit
+| CTpair ty1 ty2 : constr_type Cpair      [ADT ty1; ADT ty2]          (Tpair ty1 ty2)
 .
 
 (* an eliminator that takes cases with types given by the first index,
@@ -34,6 +35,7 @@ Inductive elim : list type -> type -> type -> Type :=
 | ENat : forall ty, elim [ty; Arrow (ADT Tnat) (Arrow ty ty)] (ADT Tnat) ty
 | EList : forall tyA ty, elim [ty; Arrow (ADT tyA) (Arrow (ADT (Tlist tyA)) (Arrow ty ty))] (ADT (Tlist tyA)) ty
 | EUnit : forall ty, elim [ty] (ADT Tunit) ty
+| EPair : forall ty1 ty2 ty, elim [Arrow (ADT ty1) (Arrow (ADT ty2) ty)] (ADT (Tpair ty1 ty2)) ty
 .
 
 Section expr.
@@ -68,6 +70,7 @@ Definition constr_denote {arg_tys ty c} (ct : constr_type c arg_tys ty) :
   | CTnil _ => fun _ => []
   | CTcons _ => fun h => cons (hhead h) (hhead (htail h))
   | CTtt => fun _ => tt
+  | CTpair _ _ => fun h => (hhead h, hhead (htail h))
   end.
 
 
@@ -78,6 +81,7 @@ Definition elim_denote {case_tys target_ty ty} (e : elim case_tys target_ty ty) 
   | ENat _ => fun cases target => (nat_rect _ (hhead cases) (hhead (htail cases)) target)
   | EList _ _ => fun cases target => (list_rect _ (hhead cases) (hhead (htail cases)) target)
   | EUnit _ => fun cases target => unit_rect _ (hhead cases) target
+  | EPair _ _ _ => fun cases target => prod_rect _ (hhead cases) target
   end.
 
 Definition expr_mut_rect
@@ -153,12 +157,17 @@ Ltac typename_reflect' x :=
   match x with
   | nat => constr:(Tnat)
   | bool => constr:(Tbool)
-  | list ?X => let r := typename_reflect' X in constr:(Tlist r)
   | unit => constr:(Tunit)
+  | list ?X => let r := typename_reflect' X in constr:(Tlist r)
+  | prod ?X ?Y => let rX := typename_reflect' X in
+                 let rY := typename_reflect' Y in
+                 constr:(Tpair rX rY)
+
   end.
 Ltac typename_reflect x := let r := typename_reflect' x in exact r.
 
 Check ltac:(typename_reflect (list (list (list unit)))).
+Check ltac:(typename_reflect (unit * bool * unit * nat * list bool)%type).
 
 Ltac type_reflect' x :=
   match x with
@@ -204,6 +213,11 @@ Ltac reflect' x :=
     let r1 := reflect' X in
     let r2 := reflect' Y in
     uconstr:(Constr (CTcons _) (hcons r1 (hcons r2 hnil)))
+  | fun (x : ?T) => @pair ?tyA ?tyB (@?X x) (@?Y x) =>
+    let r1 := reflect' X in
+    let r2 := reflect' Y in
+    uconstr:(Constr (CTpair _ _) (hcons r1 (hcons r2 hnil)))
+
   | fun (x : ?T) => if @?B x then @?X x else @?Y x =>
     let r1 := reflect' B in
     let r2 := reflect' X in
@@ -219,6 +233,11 @@ Ltac reflect' x :=
     let r2 := reflect' Y in
     let r3 := reflect' l in
     uconstr:(Elim (EList _ _) (hcons r1 (hcons r2 hnil)) r3)
+  | fun (x : ?T) => @prod_rect ?A ?B _ (@?X x) (@?p x) =>
+    let r1 := reflect' X in
+    let r2 := reflect' p in
+    uconstr:(Elim (EPair _ _ _) (hcons r1 hnil) r2)
+
   | fun (x : ?T) (y : ?A) => @?E x y =>
     let rA := type_reflect' A in
     let r := reflect' (fun (p : T * A) => E (fst p) (snd p)) in
@@ -242,6 +261,7 @@ Check ltac:(reflect (fun _ : nat => (S O)))  : expr [] _ .
 Check ltac:(reflect (fun x : nat => (S x)))  : expr [] _ .
 Check ltac:(reflect (fun x : bool => x))  : expr [] _ .
 Check ltac:(reflect (fun f : bool -> bool => f))  : expr [] _ .
+Check ltac:(reflect (tt, true))  : expr [] _ .
 Check ltac:(reflect ((S O) :: nil))  : expr [] _ .
 Check ltac:(reflect [1; 2; 3])  : expr [] _ .
 Check ltac:(reflect [true; false])  : expr [] _ .
@@ -255,7 +275,7 @@ Eval compute in expr_denote ltac:(reflect  (@list_rect nat (fun _ => list nat) [
 Check ltac:(reflect (@list_rect bool (fun _ => list bool) [] (fun h _ t => cons false (cons h t)) [true; true; true])) : expr [] _ .
 Eval compute in expr_denote (ltac:(reflect (@list_rect bool (fun _ => list bool) [] (fun h _ t => cons false (cons h t)) [true; true; true]))) hnil.
 Check ltac:(reflect (fun (x _ _ _ _ _ _ _ _ _ _ : nat) => x))  : expr [] _ .
-
+Check ltac:(reflect (@prod_rect nat nat (fun _ => nat) (fun a b => a) (1, 3)))  : expr [] _ .
 
 Section tests.
 
@@ -462,6 +482,7 @@ refine match e with
          | ENat t     => _
          | EList _ t => _
          | EUnit t    => _
+         | EPair _ _ t => _
        end.
 
 Definition eliminate {case_tys target_tyn arg_tys ty l c}
@@ -492,6 +513,9 @@ Definition eliminate {case_tys target_tyn arg_tys ty l c}
      exact match ct with
             | CTtt => fun _ => hhead cases
             end.
+   - refine match ct with
+            | CTpair _ _ => fun cases args => App (App (hhead cases) (hhead args)) (hhead (htail args))
+            end.
 Defined.
 
 Fixpoint arrow_all (ty_rec : type) (arg_rec : type) (args : list type) (dest : type) : type :=
@@ -507,17 +531,37 @@ Fixpoint arrow_all (ty_rec : type) (arg_rec : type) (args : list type) (dest : t
 Fixpoint type_size (tyn : type_name) : nat :=
   match tyn with
   | Tlist tyn' => S (type_size tyn')
+  | Tpair ty1 ty2 => S (type_size ty1 + type_size ty2)
   | _ => 1
   end.
 
-Lemma no_infinite_types :
-  forall ty, ty =Tlist ty -> False.
+Lemma no_infinite_types_list :
+  forall ty, ty = Tlist ty -> False.
 Proof.
   intros.
   apply f_equal with (f := type_size) in H.
   simpl in *.
   omega.
 Qed.
+
+Lemma no_infinite_types_pair1 :
+  forall ty1 ty2, ty1 = Tpair ty1 ty2 -> False.
+Proof.
+  intros.
+  apply f_equal with (f := type_size) in H.
+  simpl in *.
+  omega.
+Qed.
+
+Lemma no_infinite_types_pair2 :
+  forall ty1 ty2, ty2 = Tpair ty1 ty2 -> False.
+Proof.
+  intros.
+  apply f_equal with (f := type_size) in H.
+  simpl in *.
+  omega.
+Qed.
+
 
 Definition eliminate_case_type
            {case_tys target_tyn arg_tys c ty}
@@ -544,12 +588,20 @@ Definition eliminate_case_type
     + exact Here.
     + simpl.
       repeat break_if; try congruence.
-      * inv e0. exfalso. eauto using no_infinite_types.
+      * inv e0. exfalso. eauto using no_infinite_types_list.
       * exact (There Here).
   - refine match ct with
            | CTtt => _
            end.
     + exact (Here).
+  - refine match ct with
+           | CTpair _ _ => _
+           end.
+    simpl. break_if.
+    + exfalso. inv e0. eauto using no_infinite_types_pair1.
+    + break_if.
+      * exfalso. inv e0. eauto using no_infinite_types_pair2.
+      * exact Here.
 Defined.
 
 Fixpoint unroll {l ty_rec arg_rec arg_tys ty}
@@ -588,9 +640,14 @@ Proof.
   dependent destruction e; dependent destruction ct; intros;
   repeat dependent destruction args;
   repeat dependent destruction cases; auto.
-  simpl. repeat break_match; try congruence.
-  - exfalso. inv e. eauto using no_infinite_types.
-  - dependent destruction e. auto.
+  - simpl. repeat break_match; try congruence.
+    + exfalso. inv e. eauto using no_infinite_types_list.
+    + dependent destruction e. auto.
+  - simpl. repeat break_match; try congruence.
+    + exfalso. inv e. eauto using no_infinite_types_pair1.
+    + exfalso. inv e. eauto using no_infinite_types_pair1.
+    + exfalso. inv e. eauto using no_infinite_types_pair2.
+    + auto.
 Qed.
 
 Theorem eliminate_denote :
@@ -631,6 +688,12 @@ Proof.
            | CTtt => _
            end; simpl; intros;
     repeat destruct cases as [? cases] using case_hlist_cons;
+      simpl; auto.
+  - refine match ct with
+           | CTpair _ _ => _
+           end; simpl; intros;
+    repeat destruct cases as [? cases] using case_hlist_cons;
+    repeat destruct args as [? args] using case_hlist_cons;
       simpl; auto.
 Qed.
 
